Fixed Domain and Values HAppend instances and stubbed out the iff proofs for annotated syntax.  There still seems to be an issue with the Args semantics, likely related to how the common domain is defined.

Total/Stlc/Lang/Annotated/Grammar.lean
@@ -11,28 +11,24 @@ namespace Total.Stlc.Lang.Annotated
 
     inductive Domain: Nat → Type where
       | nil (τ: Ty): Domain 1
-      | cons {α: Nat} (τ: Ty) (rest: Domain α): Domain α.succ
+      | cons {α: Nat} (τ: Ty) (rest: Domain α): Domain (1 + α)
   end
 
-  @[reducible]
-  instance: {α β: Nat} → HAppend (Domain α) (Domain β) (Domain (β + α)) where
+  instance: {α β: Nat} → HAppend (Domain α) (Domain β) (Domain (α + β)) where
     hAppend lhs rhs :=
       append lhs rhs
       where
-        @[reducible]
-        append {α β: Nat}: Domain α → Domain β → Domain (β + α)
-          | .nil τ,       δ => .cons τ δ
-          | .cons τ rest, δ => .cons τ (append rest δ)
+        append {α β: Nat}: Domain α → Domain β → Domain (α + β)
+          | .nil τ,     δ₂ => Nat.add_comm _ _              ▸ .cons τ δ₂
+          | .cons τ δ₁, δ₂ => Eq.symm (Nat.add_assoc 1 _ _) ▸ .cons τ (append δ₁ δ₂)
 
-  @[reducible]
   instance: {α: Nat} → HAppend (Domain α) Ty (Domain (α + 1)) where
     hAppend lhs rhs :=
       append lhs rhs
       where
-        @[reducible]
         append {α: Nat}: Domain α → Ty → Domain (α + 1)
-          | .nil τ₁,       τ₂ => .cons τ₁ (.nil τ₂)
-          | .cons τ₁ rest, τ₂ => .cons τ₁ (append rest τ₂)
+          | .nil τ₁,    τ₂ => .cons τ₁ (.nil τ₂)
+          | .cons τ₁ δ, τ₂ => .cons τ₁ (append δ τ₂)
 
   inductive PrimOp: {α: Nat} → Domain α → Ty → Type where
     | and: PrimOp (.cons .bool (.nil .bool)) .bool
@@ -74,17 +70,6 @@ namespace Total.Stlc.Lang.Annotated
       | values {α: Nat} {δ: Domain α} (vs: Values δ): Args δ
   end
 
-  @[reducible]
-  instance: {α β: Nat} → {δ₁: Domain α} → {δ₂: Domain β} → HAppend (Values δ₁) (Values δ₂) (Values (δ₁ ++ δ₂)) where
-    hAppend lhs rhs :=
-      append lhs rhs
-      where
-        @[reducible]
-        append {α β: Nat} {δ₁: Domain α} {δ₂: Domain β}: Values δ₁ → Values δ₂ → Values (δ₁ ++ δ₂)
-          | .nil v,       vs => .cons v vs
-          | .cons v rest, vs => .cons v (append rest vs)
-
-  @[reducible]
   instance: {α: Nat} → {δ: Domain α} → {τ: Ty} → HAppend (Values δ) (Value τ) (Values (δ ++ τ)) where
     hAppend lhs rhs :=
       append lhs rhs
